code/experimental/rsa/Hacl.Impl.Montgomery.fst
@@ -16,247 +16,138 @@ open Hacl.Impl.Shift
 module Buffer = Spec.Lib.IntBuf
 
 val bn_pow2_mod_n_:
-    #rLen:size_nat ->
-    rrLen:size_t{v rrLen == rLen} -> a:lbignum rLen ->
-    i:size_t -> p:size_t ->
-    res:lbignum rLen -> Stack unit
+  #rLen:size_nat -> rrLen:size_t{v rrLen == rLen} ->
+  a:lbignum rLen -> i:size_t -> p:size_t ->
+  res:lbignum rLen -> 
+  Stack unit
     (requires (fun h -> live h a /\ live h res /\ disjoint res a))
     (ensures (fun h0 _ h1 -> preserves_live h0 h1 /\ modifies1 res h0 h1))
-    [@"c_inline"]
-let rec bn_pow2_mod_n_ #rLen clen a i p res =
-    if (i <. p) then begin
-        bn_lshift1 #rLen clen res res;
-        (if not (bn_is_less clen res clen a) then
-            bn_sub clen res clen a res);
-        bn_pow2_mod_n_ clen a (size_incr i) p res
-    end
+  [@"c_inline"]
+let rec bn_pow2_mod_n_ #rLen rrLen a i p res =
+  if (i <. p) then begin
+    bn_lshift1 #rLen rrLen res res;
+    (if not (bn_is_less rrLen res rrLen a) then
+      bn_sub rrLen res rrLen a res);
+    bn_pow2_mod_n_ rrLen a (size_incr i) p res
+  end
 
 // res = 2 ^^ p % a
 val bn_pow2_mod_n:
-    #rLen:size_nat ->
-    aBits:size_t ->
-    rrLen:size_t{v rrLen == rLen /\ v aBits / 64 < rLen} -> a:lbignum rLen ->
-    p:size_t{v aBits < v p} ->
-    res:lbignum rLen -> Stack unit
+  #rLen:size_nat ->
+  aBits:size_t ->
+  rrLen:size_t{v rrLen == rLen /\ v aBits / 64 < rLen} -> a:lbignum rLen ->
+  p:size_t{v aBits < v p} ->
+  res:lbignum rLen ->
+  Stack unit
     (requires (fun h -> live h a /\ live h res /\ disjoint res a))
     (ensures (fun h0 _ h1 -> preserves_live h0 h1 /\ modifies1 res h0 h1))
-    [@"c_inline"]
-let bn_pow2_mod_n #rLen aBits rLen a p res =
-    bn_set_bit rLen res aBits;
-    bn_sub rLen res rLen a res; // res = res - a
-    bn_pow2_mod_n_ rLen a aBits p res
+  [@"c_inline"]
+let bn_pow2_mod_n #rLen aBits rrLen a p res =
+  bn_set_bit rrLen res aBits;
+  bn_sub rrLen res rrLen a res; // res = res - a
+  bn_pow2_mod_n_ rrLen a aBits p res
 
-val degree_:
-    #aLen:size_nat ->
-    aaLen:size_t{v aaLen == aLen} ->
-    a:lbignum aLen ->
-    i:size_t{v i / 64 < aLen} -> Stack size_t
-    (requires (fun h -> live h a))
-    (ensures (fun h0 _ h1 -> preserves_live h0 h1 /\ h0 == h1))
-    [@"c_inline"]
-let rec degree_ #aLen aaLen a i =
-    if i =. size 0 then size 0
-    else begin
-       if (bn_is_bit_set aaLen a (size_decr i)) then i
-       else degree_ aaLen a (size_decr i)
-    end
+(*
+  for (size_t i = 0; i < 64; ++i) {
+    uint64_t u_is_odd = 0uL - (u & 1); /* Either 0xff..ff or 0. */
+    uint64_t beta_if_u_is_odd = beta & u_is_odd; /* Either |beta| or 0. */
+    u = ((u ^ beta_if_u_is_odd) >> 1) + (u & beta_if_u_is_odd);
 
-val degree:
-    #aLen:size_nat ->
-    aaLen:size_t{v aaLen == aLen} ->
-    a:lbignum aLen ->
-    aBits:size_t{v aBits / 64 < aLen} -> Stack size_t
-    (requires (fun h -> live h a))
-    (ensures (fun h0 _ h1 -> preserves_live h0 h1 /\ h0 == h1))
-    [@"c_inline"]
-let degree #aLen aaLen a aBits = degree_ aaLen a aBits
+    uint64_t alpha_if_u_is_odd = alpha & u_is_odd; /* Either |alpha| or 0. */
+    v = (v >> 1) + alpha_if_u_is_odd;
+  }
+*)
+val mod_inv_u64_:
+  alpha:uint64 -> beta:uint64 -> ub:uint64 -> vb:uint64 -> i:size_t{v i <= 64} -> Tot uint64
+  (decreases (64 - v i))
+let rec mod_inv_u64_ alpha beta ub vb i =
+  if (i <. size 64) then begin
+    let u_is_odd = u64 0 -. (ub &. u64 1) in
+    let beta_if_u_is_odd = beta &. u_is_odd in
+    let ub = add_mod #U64 (shift_right #U64 (ub ^. beta_if_u_is_odd) (u32 1)) (ub &. beta_if_u_is_odd) in
 
-val shift_euclidean_mod_inv_f:
-    #rLen:size_nat -> rrLen:size_t{v rrLen == rLen} ->
-    m:lbignum rLen -> tmp:lbignum rLen ->
-    f:size_t -> i:size_t -> Stack unit
-    (requires (fun h -> live h m /\ live h tmp /\ disjoint m tmp))
-    (ensures (fun h0 _ h1 -> preserves_live h0 h1 /\ modifies1 tmp h0 h1))
-    [@"c_inline"]
-let rec shift_euclidean_mod_inv_f #rLen rrLen m tmp f i =
-    if (i <. f) then begin
-       bn_add rrLen tmp rrLen tmp tmp; // tmp = tmp + tmp
-       (if (bn_is_less rrLen m rrLen tmp) then // m < tmp
-           bn_sub rrLen tmp rrLen m tmp); //tmp = tmp - m
-       shift_euclidean_mod_inv_f #rLen rrLen m tmp f (size_incr i)
-    end
+    let alpha_if_u_is_odd = alpha &. u_is_odd in
+    let vb = add_mod #U64 (shift_right #U64 vb (u32 1)) alpha_if_u_is_odd in
+    mod_inv_u64_ alpha beta ub vb (size_incr i) end 
+  else vb
 
-val shift_euclidean_mod_inv_:
-    #rLen:size_nat -> rrLen:size_t{v rrLen == rLen /\ rLen + rLen < max_size_t} ->
-    du:size_t{v du / 64 < rLen} -> ub:lbignum rLen ->
-    dv:size_t{v dv / 64 < rLen /\ v dv <= v du} -> vb:lbignum rLen ->
-    r:lbignum rLen -> s:lbignum rLen ->
-    a:lbignum rLen -> m:lbignum rLen -> 
-    st_inv:lbignum (rLen + rLen) -> res:lbignum rLen -> Stack unit
-    (requires (fun h -> live h ub /\ live h vb /\ live h s /\ live h r /\
-                      live h a /\ live h m /\ live h st_inv /\ live h res /\
-		      disjoint m st_inv))
-    (ensures (fun h0 _ h1 -> preserves_live h0 h1))
-    #reset-options "--z3rlimit 50 --max_fuel 2"
-    [@"c_inline"]
-let rec shift_euclidean_mod_inv_ #rLen rrLen du ub dv vb r s a m st_inv res =
-    let stLen = add #SIZE rrLen rrLen in
-    let v_shift_f = Buffer.sub #uint64 #(v stLen) #rLen st_inv (size 0) rrLen in
-    let tmp = Buffer.sub #uint64 #(v stLen) #rLen st_inv rrLen rrLen in
-    
-    if (dv >. size 1) then begin
-       let f = sub #SIZE du dv in
-       bn_lshift rrLen vb f v_shift_f; //v_shift_f = v << f
-       let f =
-          if (bn_is_less rrLen ub rrLen v_shift_f) then begin // u < v_shift_f
-             assume (0 < v f);
-             let f = size_decr f in
-             bn_lshift rrLen vb f v_shift_f; f end
-          else f in
-       bn_sub rrLen ub rrLen v_shift_f ub; // u = u - v_shift_f
-       
-       copy rrLen s tmp;
-       assume (disjoint m tmp);
-       shift_euclidean_mod_inv_f #rLen rrLen m tmp f (size 0);
-       (if (bn_is_less rrLen r rrLen tmp) then begin // r < tmp
-            bn_add rrLen r rrLen m r; //r = r + m
-            bn_sub rrLen r rrLen tmp r end
-        else bn_sub rrLen r rrLen tmp r);
-	 
-       let du = degree rrLen ub du in
-       if (bn_is_less rrLen ub rrLen vb) 
-       then begin
-         assume (v du < v dv);
-         shift_euclidean_mod_inv_ rrLen dv vb du ub s r a m st_inv res end
-       else begin 
-         assume (v dv <= v du /\ v du / 64 < rLen);
-         shift_euclidean_mod_inv_ rrLen du ub dv vb r s a m st_inv res end
-       end
-    else begin
-       if (dv =. size 0) then
-         fill rrLen res (u64 0)
-       else copy rrLen s res
-    end
-      
-val shift_euclidean_mod_inv:
-    #rLen:size_nat -> rrLen:size_t{v rrLen == rLen /\ 6 * rLen < max_size_t} ->
-    aBits:size_t{v aBits / 64 < rLen} -> a:lbignum rLen ->
-    mBits:size_t{v mBits / 64 < rLen /\ v aBits <= v mBits} -> m:lbignum rLen ->
-    res:lbignum rLen -> Stack unit
-    (requires (fun h -> live h a /\ live h m /\ live h res))
-    (ensures (fun h0 _ h1 -> preserves_live h0 h1 /\ modifies1 res h0 h1))
-    [@"c_inline"]
-let shift_euclidean_mod_inv #rLen rrLen aBits a mBits m res =
-    let stLen = mul #SIZE (size 6) rrLen in
-    alloc #uint64 #unit #(v stLen) stLen (u64 0) [BufItem a; BufItem m] [BufItem res]
-    (fun h0 _ h1 -> True)
-    (fun st ->
-      let ub = Buffer.sub #uint64 #(v stLen) #rLen st (size 0) rrLen in
-      let vb = Buffer.sub #uint64 #(v stLen) #rLen st rrLen rrLen in
-      let r = Buffer.sub #uint64 #(v stLen) #rLen st (add #SIZE rrLen rrLen) rrLen in
-      let s = Buffer.sub #uint64 #(v stLen) #rLen st (mul #SIZE (size 3) rrLen) rrLen in
-      let st_inv = Buffer.sub #uint64 #(v stLen) #(rLen + rLen) st (mul #SIZE (size 4) rrLen) (add #SIZE rrLen rrLen) in
+val mod_inv_u64: n0:uint64 -> Tot uint64
+let mod_inv_u64 n0 =
+  let alpha = shift_left #U64 (u64 1) (u32 63) in
+  let beta = n0 in
 
-      copy rrLen m ub;
-      copy rrLen a vb;
-      s.(size 0) <- u64 1;
-      assume (disjoint m st_inv);
-      shift_euclidean_mod_inv_ #rLen rrLen mBits ub aBits vb r s a m st_inv res;
-      admit()
-    )
+  let ub = u64 1 in
+  let vb = u64 0 in
+  mod_inv_u64_ alpha beta ub vb (size 0)
 
-#reset-options "--lax"
+val mont_reduction_:
+  #rLen:size_nat -> rrLen:size_t{v rrLen == rLen /\ rLen + rLen < max_size_t} ->
+  c:lbignum (rLen + rLen) -> n:lbignum rLen -> nInv_u64:uint64 -> i:size_t -> 
+  Stack unit
+    (requires (fun h -> live h c /\ live h n /\ disjoint c n))
+    (ensures (fun h0 _ h1 -> preserves_live h0 h1 /\ modifies1 c h0 h1))
+  [@"c_inline"]
+let rec mont_reduction_ #rLen rrLen c n nInv_u64 i =
+  if (i <. rrLen) then begin
+    let ci = c.(i) in
+    let qi = mul_mod #U64 nInv_u64 ci in
+    bn_mult_by_limb_addj rrLen n qi (size 0) i (add #SIZE rrLen rrLen) (u64 0) c;
+    mont_reduction_ rrLen c n nInv_u64 (size_incr i)
+  end
 
 val mont_reduction:
-    #rLen:size_nat -> #cLen:size_nat ->
-    exp_r:size_t{0 < v exp_r /\ rLen = v exp_r / 64 + 1} ->
-    pow2_i:size_t{rLen + rLen + 4 * v pow2_i < max_size_t /\ rLen < v pow2_i} -> iLen:size_t ->
-    rrLen:size_t{v rrLen == rLen /\ 0 < rLen /\ 6 * rLen < max_size_t} ->
-    st_mont:lbignum (3 * rLen) -> st:lbignum (3 * rLen) ->
-    st_kara:lbignum (4 * v pow2_i) ->
-    ccLen:size_t{v ccLen == cLen /\ cLen = rLen + rLen} -> c:lbignum cLen ->
-    res:lbignum rLen -> Stack unit
-    (requires (fun h -> live h st_mont /\ live h c /\ live h res))
-    (ensures (fun h0 _ h1 -> preserves_live h0 h1 /\ modifies1 res h0 h1))
-    #reset-options "--z3rlimit 50 --max_fuel 0 --max_ifuel 0"
-    [@"c_inline"]
-let mont_reduction #rLen #cLen pow2_i iLen exp_r rrLen st_mont st st_kara ccLen c res =
-    let r2Len = add #SIZE rrLen rrLen in
-    let stLen = mul #SIZE (size 3) rrLen in
-    
-    let tmp1 = Buffer.sub #uint64 #(v stLen) #(v r2Len) st (size 0) r2Len in
-    let m = Buffer.sub #uint64 #(v stLen) #rLen st r2Len rrLen in
-      
-    let r = Buffer.sub #uint64 #(v stLen) #rLen st_mont (size 0) rrLen in
-    let n = Buffer.sub #uint64 #(v stLen) #rLen st_mont rrLen rrLen in
-    let nInv = Buffer.sub #uint64 #(v stLen) #rLen st_mont r2Len rrLen in
-
-    let c1 = Buffer.sub #uint64 #cLen #rLen c (size 0) rrLen in
-    karatsuba #rLen pow2_i iLen rrLen c1 nInv st_kara tmp1; // tmp1 = c1 * nInv
-    bn_mod_pow2_n r2Len tmp1 exp_r rrLen m; // m = tmp1 % r
-    bn_sub rrLen r rrLen m m; // m = r - m
-    karatsuba #rLen pow2_i iLen rrLen m n st_kara tmp1; // tmp1 = m * n
-    bn_add r2Len tmp1 ccLen c tmp1; // tmp1 = c + tmp1
-    bn_rshift r2Len tmp1 exp_r tmp1; // tmp1 = tmp1 / r
-
-    let tmp1_ = Buffer.sub #uint64 #(v r2Len) #rLen tmp1 (size 0) rrLen in
-    copy rrLen tmp1_ res
+  #rLen:size_nat -> rrLen:size_t{v rrLen == rLen /\ rLen + rLen < max_size_t} ->
+  n:lbignum rLen -> nInv_u64:uint64 ->
+  c:lbignum (rLen + rLen) -> tmp:lbignum (rLen + rLen) -> res:lbignum rLen ->
+  Stack unit
+    (requires (fun h -> live h n /\ live h c /\ live h tmp /\ live h res /\ disjoint tmp n))
+    (ensures (fun h0 _ h1 -> preserves_live h0 h1 /\ modifies2 res tmp h0 h1))
+  [@"c_inline"]
+let mont_reduction #rLen rrLen n nInv_u64 c tmp res =
+  let rLen2 = add #SIZE rrLen rrLen in
+  copy rLen2 c tmp;
+  mont_reduction_ rrLen tmp n nInv_u64 (size 0);
+  //bn_rshift rLen2 tmp (mul #SIZE (size 64) rrLen) tmp; // tmp = tmp / r
+  let tmp' = Buffer.sub #uint64 #(v rLen2) #rLen tmp rrLen rrLen in
+  copy rrLen tmp' res
 
 val to_mont:
-    #rLen:size_nat ->
-    pow2_i:size_t{rLen + rLen + 4 * v pow2_i < max_size_t /\ rLen < v pow2_i} -> iLen:size_t ->
-    exp_r:size_t{0 < v exp_r /\ rLen = v exp_r / 64 + 1} ->
-    rrLen:size_t{v rrLen == rLen /\ 0 < rLen /\ 6 * rLen < max_size_t} ->
-    st_mont:lbignum (3 * rLen) -> st:lbignum (5 * rLen) ->
-    st_kara:lbignum (4 * v pow2_i) ->
-    r2:lbignum rLen -> a:lbignum rLen ->
-    aM:lbignum rLen -> Stack unit
-    (requires (fun h -> live h st_mont /\ live h r2 /\ live h a /\ live h aM))
-    (ensures (fun h0 _ h1 -> preserves_live h0 h1 /\ modifies1 aM h0 h1))
+  #rLen:size_nat -> rrLen:size_t{v rrLen == rLen /\ rLen + rLen < max_size_t} ->
+  pow2_i:size_t{2 * rLen + 4 * v pow2_i < max_size_t /\ rLen < v pow2_i} -> 
+  iLen:size_t{v iLen < v pow2_i / 2 /\ v iLen + rLen = v pow2_i} ->
+  n:lbignum rLen -> nInv_u64:uint64 ->
+  r2:lbignum rLen -> a:lbignum rLen -> 
+  st_kara:lbignum (2 * rLen + 4 * v pow2_i) -> aM:lbignum rLen ->
+  Stack unit
+    (requires (fun h -> live h n /\ live h r2 /\ live h a /\ live h aM /\ live h st_kara))
+    (ensures (fun h0 _ h1 -> preserves_live h0 h1))
+  [@"c_inline"]
+let to_mont #rLen rrLen pow2_i iLen n nInv_u64 r2 a st_kara aM =
+  let cLen = add #SIZE rrLen rrLen in
+  let stLen = add #SIZE cLen (mul #SIZE (size 4) pow2_i) in
+  
+  let c = Buffer.sub #uint64 #(v stLen) #(v cLen) st_kara (size 0) cLen in
+  let st_kara' = Buffer.sub #uint64 #(v stLen) #(4 * v pow2_i) st_kara cLen (mul #SIZE (size 4) pow2_i) in
+  assume (disjoint c a /\ disjoint c r2 /\ disjoint st_kara' a /\ disjoint st_kara' r2);
+  karatsuba #rLen pow2_i iLen rrLen a r2 st_kara' c; // c = a * r2
+  assume (disjoint c n);
+  mont_reduction #rLen rrLen n nInv_u64 c c aM // aM = c % n
 
-#reset-options "--z3rlimit 50 --max_fuel 0 --max_ifuel 0"
-    [@"c_inline"]
-let to_mont #rLen pow2_i iLen exp_r rrLen st_mont st st_kara r2 a aM =
-    let cLen = add #SIZE rrLen rrLen in
-    let stLen = mul #SIZE (size 3) rrLen in
-    
-    let c = Buffer.sub #uint64 #(5 * rLen) #(v cLen) st (size 0) cLen in
-    let st = Buffer.sub #uint64 #(5 * rLen) #(3 * rLen) st cLen stLen in
-    
-    karatsuba #rLen pow2_i iLen rrLen a r2 st_kara c; // c = a * r2 
-    mont_reduction pow2_i iLen exp_r rrLen st_mont st st_kara cLen c aM //aM = c % n
-    
-    
 val from_mont:
-    #rLen:size_nat ->
-    pow2_i:size_t{rLen + rLen + 4 * v pow2_i < max_size_t /\ rLen < v pow2_i} -> iLen:size_t ->
-    exp_r:size_t{0 < v exp_r /\ rLen = v exp_r / 64 + 1} ->
-    rrLen:size_t{v rrLen == rLen /\ 0 < rLen /\ 6 * rLen < max_size_t} ->
-    st_mont:lbignum (3 * rLen) -> st:lbignum (3 * rLen) ->
-    st_kara:lbignum (4 * v pow2_i) ->
-    aM:lbignum rLen -> a:lbignum rLen -> Stack unit
-    (requires (fun h ->  live h st_mont /\ live h aM /\ live h a))
-    (ensures (fun h0 _ h1 -> preserves_live h0 h1 /\ modifies1 a h0 h1))
+  #rLen:size_nat -> rrLen:size_t{v rrLen == rLen /\ rLen + rLen < max_size_t} ->
+  pow2_i:size_t{2 * rLen + 4 * v pow2_i < max_size_t /\ rLen < v pow2_i} -> 
+  iLen:size_t{v iLen < v pow2_i / 2 /\ v iLen + rLen = v pow2_i} ->
+  n:lbignum rLen -> nInv_u64:uint64 ->
+  aM:lbignum rLen -> st:lbignum (rLen + rLen) -> a:lbignum rLen ->
+  Stack unit
+    (requires (fun h -> live h n /\ live h a /\ live h aM /\ live h st))
+    (ensures (fun h0 _ h1 -> preserves_live h0 h1))
+  [@"c_inline"]
+let from_mont #rLen rrLen pow2_i iLen n nInv_u64 aM st a =
+  let rLen2 = add #SIZE rrLen rrLen in
+  fill rLen2 st (u64 0);
+  let st' = Buffer.sub #uint64 #(v rLen2) #rLen st (size 0) rrLen in
+  copy rrLen aM st';
+  assume (disjoint st n);
+  mont_reduction #rLen rrLen n nInv_u64 st st a // a = aM % n
 
-#reset-options "--z3rlimit 50 --max_fuel 0 --max_ifuel 0"
-    [@"c_inline"]
-let from_mont #rLen pow2_i iLen exp_r rrLen st_mont st st_kara aM a =
-    let r2Len = add #SIZE rrLen rrLen in
-    let stLen = mul #SIZE (size 3) rrLen in
-    
-    let tmp = Buffer.sub #uint64 #(v stLen) #(v r2Len) st (size 0) r2Len in
-    let m = Buffer.sub #uint64 #(v stLen) #rLen st r2Len rrLen in
-
-    let r = Buffer.sub #uint64 #(v stLen) #rLen st_mont (size 0) rrLen in
-    let n = Buffer.sub #uint64 #(v stLen) #rLen st_mont rrLen rrLen in
-    let nInv = Buffer.sub #uint64 #(v stLen) #rLen st_mont r2Len rrLen in
-      
-    karatsuba #rLen pow2_i iLen rrLen aM nInv st_kara tmp; // tmp = aM * nInv
-    bn_mod_pow2_n r2Len tmp exp_r rrLen m; // m = tmp % r
-    bn_sub rrLen r rrLen m m; // m = r - m
-    karatsuba #rLen pow2_i iLen rrLen m n st_kara tmp; // tmp = m * n
-    bn_add r2Len tmp rrLen aM tmp; //tmp = aM + tmp
-    bn_rshift r2Len tmp exp_r tmp; //tmp = tmp / r
-      
-    let tmp_ = Buffer.sub #uint64 #(v r2Len) #rLen tmp (size 0) rrLen in
-    copy rrLen tmp_ a
